\documentclass[conference,a4paper,onecolumn]{IEEEtran}
\usepackage{fontspec}
\usepackage[fleqn]{amsmath}
\usepackage{graphicx}
\usepackage{footnote}
\makesavenoteenv{tabular}
\usepackage{booktabs}
\usepackage{amssymb}
\usepackage{multirow}
\usepackage{makecell}
\usepackage[vlined, ruled, linesnumbered]{algorithm2e}
\usepackage{multirow}

\ifCLASSINFOpdf
\else
\fi

% correct bad hyphenation here
\hyphenation{op-tical net-works semi-conduc-tor}

\begin{document}

\begin{equation}
f_i = BE_i^{spd} Pr_{spd} + \sum \limits_{j=1} ^{N} BE_{ij} Pr_{pd} - \sum \limits_{j=1} ^{N} SE_{ij} (Pr_{pd} + Pr_{ij}).
\end{equation}
\begin{flalign}
\nonumber F = \sum \limits_{i=1} ^N f_i = \sum \limits_{i=1}^N BE_i^{spd} Pr_{spd} + \sum \limits_{i=1}^N \sum \limits_{j=1} ^{N} BE_{ij} Pr_{pd} - \sum \limits_{i=1}^N\sum \limits_{j=1} ^{N} SE_{ij} (Pr_{pd} + Pr_{ij}) \\
\nonumber = \sum \limits_{i=1}^N BE_i^{spd} Pr_{spd} - \sum \limits_{i=1}^N\sum \limits_{j=1} ^{N} SE_{ij} Pr_{ij}\\
 = \sum \limits_{i=1}^N BE_i^{spd} Pr_{spd} - \sum \limits_{i=1}^N\sum \limits_{j=1} ^{N} BE_{ij} Pr_{ij}\\
\nonumber subject\ to: \sum \limits_{i=1}^N BE_i^{spd} + \sum \limits_{i=1}^N\sum \limits_{j=1} ^{N} BE_{ij} = E_0\\
\sum \limits_{j=1}^N SE_{ij} \le (RE_i + PE_i) - CE_i^{s}\\
\sum \limits_{i=1}^N \sum \limits_{j=1}^N SE_{ij} \le \sum \limits_{i=1}^N (RE_i + PE_i) - CE_i^{s}
\end{flalign}
Equation (2) would have:
\begin{flalign}
\nonumber F = ( E_0 -\sum \limits_{i=1}^N\sum \limits_{j=1} ^{N} BE_{ij}) Pr_{spd} - \sum \limits_{i=1}^N\sum \limits_{j=1} ^{N} BE_{ij} Pr_{ij}\\
=   E_0 Pr_{spd} - \sum \limits_{i=1}^N\sum \limits_{j=1} ^{N} BE_{ij} (Pr_{spd} + Pr_{ij}) 
\end{flalign}
Therefore:
\begin{flalign}
Min\ F = Min\ ( E_0 Pr_{spd} - \sum \limits_{i=1}^N\sum \limits_{j=1} ^{N} BE_{ij} (Pr_{spd} + Pr_{ij}) )\\
\nonumber =  E_0 Pr_{spd} - Max\ \sum \limits_{i=1}^N\sum \limits_{j=1} ^{N} BE_{ij} (Pr_{spd} + Pr_{ij})\\
=  E_0 Pr_{spd} - Max\ \sum \limits_{j=1}^N\sum \limits_{i=1} ^{N} SE_{ji} (Pr_{spd} + Pr_{ji})
\end{flalign}
According to (4), equation (7) would have a mininum if and only if:
\begin{flalign}
 \sum  \limits_{i=1}^N \sum  \limits_{j=1}^N SE_{ij} = \sum \limits_{i=1}^N (RE_i + PE_i) - CE_i^{s}
\end{flalign}
\end{document}
